\documentclass[11pt]{article}

\usepackage{amsmath, amssymb}
\usepackage{xcolor}
\usepackage{tcolorbox}
\usepackage{hyperref}
\tcbset{colback=white}

\newcommand{\EE}{E\overline{E}}

\begin{document}

\section*{Solving \texorpdfstring{$aE\overline{E} + b\overline{E} + c = 0$}{aE E* + bE* + c = 0}}

We want to determine, for which triples $(a,b,c)\in\mathbb{C}^3$, the equation
\[
a\,E\overline{E} \;+\; b\,\overline{E} \;+\; c \;=\; 0
\]
admits a solution $E\in\mathbb{C}$.

% ------------------------------------------------------------
\subsection*{The case \texorpdfstring{$a=0$}{a=0}}

When $a=0$, the equation reduces to
\[
b\,\overline{E} + c = 0.
\]

\begin{tcolorbox}
\[
\text{If } b\neq 0, \qquad
\overline{E} = -\frac{c}{b}
\quad\Longrightarrow\quad
E = -\overline{\frac{c}{b}}.
\]
So a solution always exists, for every $c\in\mathbb{C}$.
\end{tcolorbox}

\smallskip

\begin{tcolorbox}
If $b = 0$, then the equation is simply $c=0$.

\begin{itemize}
    \item If $b=0$ and $c=0$: every $E$ is a solution.
    \item If $b=0$ and $c\neq 0$: no solution exists.
\end{itemize}
\end{tcolorbox}

Thus for $a=0$, a solution exists unless
\[
(b,c) = (0,k) \text{ for } k\neq 0.
\]

\bigskip

% ------------------------------------------------------------
\subsection*{From now on, assume \texorpdfstring{$a\neq 0$}{a â‰  0}}

We divide the original equation by $a$ and define
\[
b' = \frac{b}{a},
\qquad
c' = \frac{c}{a},
\]
so the equation becomes
\[
E\overline{E} + b'\,\overline{E} + c' = 0.
\]

\begin{tcolorbox}
Rewrite as
\[
c' = -\,\EE + b'\,\overline{E}.
\]
\end{tcolorbox}

Let us decompose $E$ into magnitude and direction:
\[
E = E_{\text{size}}\,E_{\text{dir}},
\qquad
|E_{\text{dir}}|=1.
\]
Then
\[
c' = -\,E_{\text{size}}^2 \;+\; b' E_{\text{size}}\,\overline{E_{\text{dir}}}.
\]

\smallskip

For fixed $E_{\text{size}}$, as we vary $E_{\text{dir}}$ over the unit circle,
the term $b' E_{\text{size}}\,\overline{E_{\text{dir}}}$ traces out a circle of radius $|b'| E_{\text{size}}$ centered at the origin.
Write $b_{\text{size}} = |b'|$.
Then $c'$ traces out a circle of radius $b_{\text{size}} E_{\text{size}}$ centered at $-E_{\text{size}}^2$,
which lies on the real axis.
Writing $c' = c_x + i c_y$, we have
\[
(c_x + E_{\text{size}}^2)^2 + c_y^2 = (b_{\text{size}} E_{\text{size}})^2.
\]

\bigskip

% ------------------------------------------------------------
\subsection*{Finding the envelope of these circles}

Define
\[
F(c_x,c_y,z)
  = (c_x + z^2)^2 + c_y^2 - (b_{\text{size}} z)^2.
\]
The envelope of the family is obtained from
\[
F = 0,
\qquad
\frac{\partial F}{\partial z} = 0.
\]
We have
\[
\frac{\partial F}{\partial z}
  = 2(c_x + z^2)(2z) - 2 b_{\text{size}}^2\, z
  = 2z\bigl(2(c_x + z^2) - b_{\text{size}}^2\bigr),
\]
so the envelope occurs where either $z = 0$ or $2(c_x + z^2) = b_{\text{size}}^2$.

For $z = 0$: substituting into $F=0$ gives $c_x^2 + c_y^2 = 0$, so $(c_x, c_y) = (0,0)$.

For $2(c_x + z^2) = b_{\text{size}}^2$: we have $z^2 = \frac{b_{\text{size}}^2}{2} - c_x$.
Substituting into $F=0$ gives
\[
\left(\frac{b_{\text{size}}^2}{2}\right)^2 + c_y^2 = b_{\text{size}}^2\left(\frac{b_{\text{size}}^2}{2} - c_x\right),
\]
which simplifies to
\[
c_y^2 = \frac{b_{\text{size}}^4}{4} - b_{\text{size}}^2 c_x.
\]
Since $z$ must be real, we require $z^2 = \frac{b_{\text{size}}^2}{2} - c_x \geq 0$, giving the constraint
\[
c_x \leq \frac{b_{\text{size}}^2}{2}.
\]

\begin{figure}[h]
\centering
\includegraphics[width=0.8\textwidth]{../a-complex-equation-envelope.png}
\end{figure}

\begin{tcolorbox}
\[
\boxed{
\begin{array}{c}
\text{The set of } c' \text{ for which a solution } E \text{ exists} \\
\text{is the interior of this envelope.}
\end{array}
}
\]
\end{tcolorbox}

Translating back to $c = a c'$ determines all triples $(a,b,c)$ for which a solution exists.

\end{document}
